\section{2022 Stats August Answers}
\subsection{2.3}
% Starting with our definition of convergence in distribution.  We define:
% \[
% F_{X_n}=P(\{\omega:X_n \leq x\}) \quad \text{and} \quad F_{X}=P(\{\omega:X \leq x\})
% \]
% Because \(X\) has a continuous distribution function:
% \begin{align*}
%     \lim_{n\rightarrow\infty} P(\{\omega:X_n \leq x\}) = P(\{\omega:X \leq x\}) \quad \forall\; x\in {\Bbb R} \\
%     \Leftrightarrow \lim_{n\rightarrow\infty} P(\{\omega:X_n \leq x\}) - P(\{\omega:X \leq x\}) =0 \quad \forall\; x\in {\Bbb R} \\
%     \Rightarrow \lim_{n\rightarrow\infty} |P(\{\omega:X_n \leq x\}) - P(\{\omega:X \leq x\})| =0 \quad \forall\; x\in {\Bbb R}
% \end{align*}
% This implies uniform convergence. Or that \(\forall \; \varepsilon > 0,\; \exists \; n\geq n_0 \in \; {\Bbb N}\) such that:
% \begin{align*}
%     \sup_{x \in {\Bbb R}}|P(\{\omega:X_{n\geq n_0} \leq x\}) - P(\{\omega:X \leq x\})| <\varepsilon \\
%     \text{Letting } \varepsilon\rightarrow0\text{, we have that:} \\
%     \sup_{x \in {\Bbb R}} |P(\{\omega:X_n \leq x\}) - P(\{\omega:X \leq x\})| \rightarrow 0
% \end{align*}
% As desired.