\section{2018 Metric January Answers}
\subsection{1.b}
The sum of squared residuals for the restricted model, \(y=\beta X+u\), is: \(u'u=(M_Xy)'(M_Xy) = y'M_Xy\).\\
Let \(W=[x,z]\), and let \(\phi'=[\beta_1,\gamma]\).  The sum of squared residuals for the unrestricted model, \(y=\phi W+u\), is: \(u'u=(M_Wy)'(M_Wy) = y'M_Wy\).  So we have:
\[
F = \frac{(y'M_Xy-y'M_Wy)r^{-1}}{y'M_wy(n-2)^{-1}}
\]
The denominator is written as we desire, so we will focus on the numerator.  Note that \(r=1\), so the numerator is:
\begin{align*}
    y'M_Xy-y'M_Wy &= y'(M_X-M_W)y \\
    &= y'[M_Xz(z'M_Xz)^{-1}z'M_X]y \\
    &= y'M_Xz(z'M_Xz)^{-1}z'M_Xz(z'M_Xz)^{-1}z'M_Xy \\
    &= [(z'M_Xz)^{-1}z'M_Xy]'z'M_Xz[(z'M_Xz)^{-1}z'M_Xy]
\end{align*}
So if \(\hat{\gamma}=(z'M_Xz)^{-1}z'M_Xy\), we have our desired result.  By the FWL theorem, \(\hat\gamma\) will be the same for the following regressions: 
\[
y=\phi W+u = \beta_1 x+\gamma z +u \quad \text{and} \quad M_Xy=M_X \gamma z+M_Xu
\]
The criterion function generated by the last regression is: \(Q(\beta)=(y-z\gamma )'M_X(y-z\gamma \).  Taking the FOCs, we have:
\begin{align*}
    z'M_X(y-z\hat{\gamma})=0 \Leftrightarrow z'M_X y=z'M_X z\hat{\gamma}\\
    \Leftrightarrow \hat{\gamma}=(z'M_Xz)^{-1}z'M_Xy \\
    \therefore F=\frac{z'M_Xz\hat{\gamma}^2}{y'M_wy(n-2)^{-1}}
\end{align*}

\subsection{1.c}
Starting from the F statistic we found:
\[
F=\frac{y'M_Xz(z'M_Xz)^{-1}z'M_Xy}{y'M_wy(n-2)^{-1}}
\]
Note that \(M_X\) is idempotent, so \(M_X M_X = M_X\).  Also note that under \(H_0\), \(M_X y =u\).  Finally note that \(\frac{y'M_Wy}{n-2} \overset{a}{=} \sigma^2\).  We can rewrite \(F\):
\begin{align*}
F \overset{a}{=} \frac{u' M_X z (z'M_Xz)^{-1}z'M_X u}{\sigma^2} = \frac{u'P_{M_X z}u}{\sigma^2} \\
= \frac{(P_{M_X z}u)'(P_{M_X z}u)}{\sigma^2} \sim \frac{\sigma^2 \chi^2_r}{\sigma^2} =\chi^2(r)
\end{align*}
And \(r=1\), so \(F\sim \chi^2(1)\).

\subsection{1.d}
We start with \(\hat{\gamma}=(z'M_Xz)^{-1}z'M_Xy\).  By substituting in the DGP for \(y\) and noting that \(H_0:\gamma_0=0\), we have:
\begin{align*}
    \hat{\gamma}&=(z'M_Xz)^{-1}z'M_Xu  \\
    \text{var}(\hat{\gamma}) &= \sigma^2(z'M_X z)^{-1} \\
    \widehat{\text{var}(\hat{\gamma})} &= \widehat{\sigma^2}(z'M_X z)^{-1} \\
    \widehat{\sigma^2}& = \frac{y'M_Wy}{n-2}
\end{align*}
The t-statistic is: \(t=\frac{\hat{\gamma}}{(\widehat{\text{var}(\hat{\gamma})})^{1/2}}\)
\begin{align*}
    \Leftrightarrow t &= \hat{\gamma} \left ( \frac{y'M_Wy}{n-2} (z'M_X z)^{-1} \right )^{-\frac{1}{2}} \\
    &= \hat{\gamma}(z'M_X z)^\frac{1}{2}\left ( \frac{y'M_Wy}{n-2}\right )^{-\frac{1}{2}} \\
    \therefore t^2 &=\frac{z'M_Xz\hat{\gamma}^2}{y'M_wy(n-2)^{-1}} =F \text{ as desired.}
\end{align*}



