\section{2020 Stats January Answers}
\subsection{1.C}
Let \(\mathcal{F}_X\) be the \(\sigma\)-algebra generated by X.  Let \(A \in \mathcal{F}_X\) and note that there exists a $B$ such that \(A=\{\omega:X(\omega) \in B\}\).  Where $B$ is any arbitrary set in the co-domain of $X$ and $Y$.  $A$ is arbitrary in \(\mathcal{F}_X\).
\begin{align*}
    \int_A Y dp = \int_\Omega Y \mathbf{I}_A dp \\
    =\int_\Omega Y \mathbf{I}_{X\in B} dp = E[Y \mathbf{I}_{X\in B}]
\end{align*}
Which by independence:
\[
= E[Y]E[\mathbf{I}_{X\in B}] = E[Y]\int_\Omega \mathbf{I}_{X\in B} dp= E[Y]\int_\Omega \mathbf{I}_{A} dp
\]
Because $A$ is arbitrary in \(\mathcal{F}_X\), we can say:
\[
= \int_A E[Y] dP
\]
So we have:
\begin{align*}
    \int_A YdP = \int_A E[Y]dP \\
    \Leftrightarrow \int_A[Y-E(Y)]dP=0
\end{align*}
Which by the definition of conditional expectation, we have that \(E(Y|X)=E(Y)\) Since A is arbitrary in \(\mathcal{F}_X\).
\subsection{2.C}
In this case,
\[
P(x_i \leq x) =
\begin{cases}
    0 & x \in (-\infty,0] \\
    \frac{x}{\theta} & x\in (0,\theta) \\
    1 & x\in [\theta, \infty)
\end{cases}
\]
And we have:
\begin{align*}
    P(\{n(\theta_n - \theta) \leq x\})
    = P(\{n(\frac{n+1}{n}M_n -\theta)\leq x \}) \\
    = P(\{(n+1)M_n - n\theta \leq x) \\
    = P(\{M_n \leq \frac{x+n\theta}{n+1}\}) \\
    = P(\{X_1 \leq \frac{x+n\theta}{n+1}\}\cup\ldots\cup\{X_n \leq \frac{x+n\theta}{n+1}\} \\
\end{align*}
Because \(X_n\) are independent of each other \(\forall \; n\in {\Bbb N} \), we have:
\begin{align*}
    P(\{X_1 \leq \frac{x+n\theta}{n+1}\})\cdot\;\ldots\; \cdot P(\{X_n \leq \frac{x+n\theta}{n+1}\})
\end{align*}
Using \(P(x_i \leq x)\) that we mentioned before, we have:
\[
= \left ( \frac{x+n\theta}{(n+1)\theta} \right)^n
\]
\[
\therefore \lim_{n\rightarrow \infty} P(n(\theta_n-\theta) \leq x) = \lim_{n\rightarrow\infty}\left ( \frac{x+n\theta}{(n+1)\theta} \right)^n
\]